More cat again

examples/Examples/Cat.lean
@@ -15,3 +15,226 @@ stop book declaration
 end Str
 
 similar datatypes Str.Stream IO.FS.Stream
+
+
+namespace Original
+
+def bufsize : USize := 20 * 1024
+
+partial def dump (stream : IO.FS.Stream) : IO Unit := do
+  let done ← stream.isEof
+  if done then
+    pure ()
+  else
+    let stdout ← IO.getStdout
+    let buf ← stream.read bufsize
+    stdout.write buf
+    dump stream
+
+def fileStream (filename : System.FilePath) : IO (Option IO.FS.Stream) := do
+  let fileExists ← filename.pathExists
+  if not fileExists then
+    let stderr ← IO.getStderr
+    stderr.putStrLn s!"File not found: {filename}"
+    pure none
+  else
+    let handle ← IO.FS.Handle.mk filename IO.FS.Mode.read
+    pure (some (IO.FS.Stream.ofHandle handle))
+
+def process (err : UInt32) (args : List String) : IO UInt32 := do
+  match args with
+    | [] => pure err
+    | "-" :: args =>
+      let stdin ← IO.getStdin
+      dump stdin
+      process err args
+    | filename :: args =>
+      let stream ← fileStream ⟨filename⟩
+      match stream with
+        | none =>
+          process 1 args
+        | some stream =>
+          dump stream
+          process err args
+
+def main (args : List String) : IO UInt32 :=
+  match args with
+    | [] => process 0 ["-"]
+    | _ =>  process 0 args
+
+end Original
+
+namespace Improved
+def bufsize : USize := 20 * 1024
+
+
+book declaration {{{ dump }}}
+  partial def dump (stream : IO.FS.Stream) : IO Unit := do
+    if (← stream.isEof) then
+      pure ()
+    else
+      (← IO.getStdout).write (← stream.read bufsize)
+      dump stream
+stop book declaration
+
+book declaration {{{ fileStream }}}
+  def fileStream (filename : System.FilePath) : IO (Option IO.FS.Stream) := do
+    if not (← filename.pathExists) then
+      (← IO.getStderr).putStrLn s!"File not found: {filename}"
+      pure none
+    else
+      let handle ← IO.FS.Handle.mk filename IO.FS.Mode.read
+      pure (some (IO.FS.Stream.ofHandle handle))
+stop book declaration
+
+
+book declaration {{{ process }}}
+def process (err : UInt32) (args : List String) : IO UInt32 := do
+  match args with
+    | [] => pure err
+    | "-" :: args =>
+      dump (← IO.getStdin)
+      process err args
+    | filename :: args =>
+      match (← fileStream ⟨filename⟩) with
+        | none =>
+          process 1 args
+        | some stream =>
+          dump stream
+          process err args
+stop book declaration
+
+def main (args : List String) : IO UInt32 :=
+  match args with
+    | [] => process 0 ["-"]
+    | _ =>  process 0 args
+end Improved
+
+example : Original.bufsize = Improved.bufsize := by rfl
+
+@[simp]
+axiom dumpEquals : Original.dump = Improved.dump
+
+@[simp]
+theorem fileStreamEquals : Original.fileStream = Improved.fileStream := by rfl
+
+@[simp]
+theorem processEqual : Original.process = Improved.process := by
+  funext err args; revert err
+  induction args with
+    | nil =>
+      simp [Original.process, Improved.process]
+    | cons head tail ih =>
+      cases decEq head "-" <;> simp [*, ih, Original.process, Improved.process]
+
+example : Original.main = Improved.main := by
+  simp [Original.main, Improved.main]
+
+
+
+
+
+book declaration {{{ getNumA }}}
+  def getNumA : IO Nat := do
+    (← IO.getStdout).putStrLn "A"
+    pure 5
+stop book declaration
+
+
+book declaration {{{ getNumB }}}
+  def getNumB : IO Nat := do
+    (← IO.getStdout).putStrLn "B"
+    pure 7
+stop book declaration
+
+book declaration {{{ getNums }}}
+  def getNums (n : Nat) : IO (Nat × Nat) := do
+    (← IO.getStdout).putStrLn "Nums"
+    pure (n, n+n)
+stop book declaration
+
+
+book declaration {{{ testEffects }}}
+  def test : IO Unit := do
+    let a : Nat := if (← getNumA) == 5 then 0 else (← getNumB)
+    (← IO.getStdout).putStrLn s!"The answer is {a}"
+stop book declaration
+
+expect info {{{ runTest }}}
+  #eval test
+message
+"A
+B
+The answer is 0
+"
+end expect
+
+namespace Foo
+book declaration {{{ testEffectsExpanded }}}
+  def test : IO Unit := do
+    let x ← getNumA
+    let y ← getNumB
+    let a : Nat := if x == 5 then 0 else y
+    (← IO.getStdout).putStrLn s!"The answer is {a}"
+stop book declaration
+end Foo
+
+example : test = Foo.test := by rfl
+
+def a : IO Nat := do
+  pure ((← getNumA) + (← getNums (← getNumB)).snd)
+
+def b : IO Nat := do
+  let x ← getNumA
+  let y ← getNumB
+  let z ← getNums y
+  pure (x + z.snd)
+
+def c : IO Nat := do
+  let y ← getNumA
+  let x ← getNumB
+  let z ← getNums y
+  pure (x + z.snd)
+
+
+def one : IO Nat := pure 1
+def two : IO Nat := pure 2
+
+namespace HelloName1
+book declaration {{{ helloOne }}}
+-- This version uses only whitespace-sensitive layout
+def main : IO Unit := do
+  let stdin ← IO.getStdin
+  let stdout ← IO.getStdout
+
+  stdout.putStrLn "How would you like to be addressed?"
+  let name := (← stdin.getLine).dropRightWhile Char.isWhitespace
+  stdout.putStrLn s!"Hello, {name}!"
+stop book declaration
+end HelloName1
+
+namespace HelloName2
+book declaration {{{ helloTwo }}}
+-- This version is as explicit as possible
+def main : IO Unit := do {
+  let stdin ← IO.getStdin;
+  let stdout ← IO.getStdout;
+
+  stdout.putStrLn "How would you like to be addressed?";
+  let name := (← stdin.getLine).dropRightWhile Char.isWhitespace;
+  stdout.putStrLn s!"Hello, {name}!"
+}
+stop book declaration
+end HelloName2
+
+namespace HelloName3
+book declaration {{{ helloThree }}}
+-- This version uses a semicolon to put two actions on the same line
+def main : IO Unit := do
+  let stdin ← IO.getStdin; let stdout ← IO.getStdout
+
+  stdout.putStrLn "How would you like to be addressed?"
+  let name := (← stdin.getLine).dropRightWhile Char.isWhitespace
+  stdout.putStrLn s!"Hello, {name}!"
+stop book declaration
+end HelloName3
