functional-programming-lean/src/hello-world/conveniences.md
@@ -1,1 +1,88 @@
 # Additional Conveniences
+
+There are a number of ways to make the `do` notation for `IO` actions more concise.
+
+## Nested Actions
+
+Many of the functions in `feline` exhibit a repetitive pattern in which an `IO` action's result is given a name, and then used immediately and only once.
+For instance, in `dump`:
+```Lean
+{{#include ../../../examples/feline/2/Main.lean:dump}}
+```
+the pattern occurs twice:
+```Lean
+{{#include ../../../examples/feline/2/Main.lean:isEofBind}}
+```
+and
+```Lean
+{{#include ../../../examples/feline/2/Main.lean:bufBind}}
+```
+Similarly, `fileStream` contains the following snippet:
+```Lean
+{{#include ../../../examples/feline/2/Main.lean:fileExistsBind}}
+```
+
+When Lean is compiling a `do` block, expressions that consist of a left arrow immediately under parentheses are lifted to the nearest enclosing `do`, and their results are bound to a unique name.
+This unique name replaces the origin of the expression.
+This means that `dump` can also be written as follows:
+```Lean
+{{#example_decl Examples/Cat.lean dump}}
+```
+This version of `dump` avoids introducing names that are used only once, which can greatly simplify a program.
+`IO` actions that Lean lifts from a nested expression context are called _nested actions_.
+
+`fileStream` can be simplified using the same technique:
+```Lean
+{{#example_decl Examples/Cat.lean fileStream}}
+```
+In this case, the local name of `handle` could also have been eliminated using nested actions, but the resulting expression would have been long and complicated.
+Even though it's often good style to use nested actions, it can still sometimes be helpful to name intermediate results.
+
+It is important to remember, however, that nested actions are only a shorter notation for `IO` actions that occur in a surrounding `do` block.
+The side effects that are involved in executing the still occur in the same order, and execution of side effects is not interspersed with the evaluation of expressions.
+For an example of where this might be confusing, consider the following helper definitions that return data after announcing to the world that they have been executed:
+```Lean
+{{#example_decl Examples/Cat.lean getNumA}}
+
+{{#example_decl Examples/Cat.lean getNumB}}
+```
+These definitions are intended to stand in for more complicated `IO` code that might validate user input, read a database, or open a file.
+
+A program that prints `0` when number A is five, or number `B` otherwise, can be written as follows:
+```Lean
+{{#example_decl Examples/Cat.lean testEffects}}
+```
+However, this program probably has more side effects (such as prompting for user input or reading a database) than was intended.
+The definition of `getNumA` makes it clear that it will always return `5`, and thus the program should not read number B.
+However, running the program results in the following output:
+```Lean info
+{{#example_out Examples/Cat.lean runTest}}
+```
+`getNumB` was executed because `test` is equivalent to this definition:
+```Lean
+{{#example_decl Examples/Cat.lean testEffectsExpanded}}
+```
+This is due to the rule that nested actions are lifted to the _closest enclosing_ `do` block.
+The branches of the `if` were not implicitly wrapped in `do` blocks because the `if` is not _immediately_ under a `do`.
+Indeed, they could not be wrapped this way, because the type of the conditional expression is `Nat`, not `IO Nat`.
+
+## Flexible Layouts for `do`
+
+In Lean, `do` expressions are whitespace-sensitive.
+Each `IO` action or local binding in the `do` is expected to start on its own line, and they should all have the same indentation.
+Almost all uses of `do` should be written this way.
+In some rare contexts, however, manual control over whitespace and indentation may be necessary, or it may be convenient to have multiple small actions on a single line.
+In these cases, newlines can be replaced with a semicolon and indentation can be replaced with curly braces.
+
+For instance, all of the following programs are equivalent:
+```Lean
+{{#example_decl Examples/Cat.lean helloOne}}
+
+{{#example_decl Examples/Cat.lean helloTwo}}
+
+{{#example_decl Examples/Cat.lean helloThree}}
+```
+
+Idiomatic Lean code uses curly braces with `do` very rarely.
+
+
