functional-programming-lean/src/hello-world/summary.md
@@ -1,1 +1,7 @@
 # Summary
+
+## Evaluation vs Execution
+
+
+
+## Compiling and Running Programs
